rupicola/io/IO.fst
@@ -40,26 +40,18 @@ let rec theta #a (m:io a) : hist a =
   | Return x -> hist_return x
   | Call o args k -> hist_bind (op_wp o args) (fun r -> theta (k r))
 
+let theta_monad_morphism_ret x =
+  assert (theta (return x) == hist_return x) by (FStar.Tactics.compute ())
+
+let theta_monad_morphism_bind m k = admit ()
+
+let wp2p_theta_bind m k =
+  theta_monad_morphism_bind m k
+
 let io_bind_equivalence (#a #b:Type) (k k':a -> io b) (m:io a) :
   Lemma (requires forall x. k x == k' x)
         (ensures theta (io_bind m k) `hist_equiv` theta (io_bind m k')) = admit ()
-        
-let lem_theta_return (#a:Type) (x:a) (h:history) (lt:local_trace h) :
-  Lemma (requires lt == [])
-        (ensures wp2p (theta (return x)) h lt x) =
-  introduce forall p. theta (return x) h p ==> p lt x with begin
-    introduce theta (return x) h p ==> p lt x with _. begin
-      assert (return x == Return x);
-      assert (theta (return x) h p == p [] x)
-    end
-  end
-
-let lem_theta_bind #a #b (m:io a) (h:history) (lt2:local_trace h) (fs_r_m:a) (k:a -> io b) (lt3:local_trace (h++lt2)) (fs_r:b) (lt:local_trace h) :
-  Lemma (requires wp2p (theta m) h lt2 fs_r_m /\
-                  wp2p (theta (k fs_r_m)) (h++lt2) lt3 fs_r /\
-                  (lt == lt2 @ lt3))
-        (ensures wp2p (theta (io_bind m k)) h lt fs_r) = admit ()
 
 let theta_history_independence #a (m:io a) (h h':history) (lt:local_trace h) (lt':local_trace h') (fs_r:a) :
-  Lemma (requires wp2p (theta m) h lt fs_r) 
+  Lemma (requires wp2p (theta m) h lt fs_r)
         (ensures wp2p (theta m) h' lt' fs_r) = admit ()
